

16 2 short questions

Ex 4c

2 i)  $(x+8)(x+10)$

$$(x+8)(x+10) = x^2 + (8+10)x + 8 \times 10 \\ = x^2 + 18x + 80$$

ii)  $(x+a)(x-b) = x^2 + (a-b)x - ab$

$$(x+8)(x-10) = x^2 + (8-10)x - 8 \times 10 \\ = x^2 - 2x - 80$$

iii)  $(x-a)(x+b) = x^2 + (b-a)x - ab$   
 $(x-8)(x-10) = x^2 + (10-8)x - 8 \times 10 \\ = x^2 + 2x - 80$

iv)  $(x-a)(x-b) = x^2 - (a+b)x + ab$   
 $(x-8)(x-10) = x^2 - (8+10)x + 8 \times 10$

Expand

i)  $\left(x - \frac{1}{7}\right)\left(3x + \frac{2}{7}\right)$

$$2a \left( \frac{3a+2}{a} \right) - \frac{1}{a} \left( \frac{3a+2}{a} \right)$$

$$\frac{6a^2 + 4a}{a} - \frac{3a}{a} - \frac{2}{a^2}$$

$$6a^2 - \frac{2}{a^2} + 1$$

ii  $\left( \frac{3a+2}{a} \right) \left( \frac{2a-3}{a} \right)$

$$3a \left( \frac{2a-3}{a} \right) + \frac{2}{a} \left( \frac{2a-3}{a} \right)$$

$$\frac{6a^2 - 9a}{a} + \frac{4a - 6}{a^2}$$

$$6a^2 - \frac{9a + 4a - 6}{a^2}$$

$$6a^2 - \frac{5a - 4}{a^2}$$

iii  $(a+b+c)^2 = a^2 + b^2 + c^2 + 2(ab+bc+ca)$

$a=x, b=y, c=-z$

$$\begin{aligned} (x+y-z)^2 &= x^2 + y^2 + (-z)^2 + 2(xy + y(-z) + (-z)x) \\ &= x^2 + y^2 + z^2 + 2(xy - yz - zx) \end{aligned}$$

$$(x+y-z)^2 = x^2 + y^2 + z^2 + 2(xy + yz - zx)$$

$$\therefore (x+y-z)^2 = x^2 + y^2 + z^2 + 2xy + 2yz - 2zx$$

ii  $a=x, b=2y, c=2$

$$(a+b+c)^2 = a^2 + b^2 + c^2 + 2(ab + bc + ca)$$

$$(x+2y+2)^2 = x^2 + (-2y)^2 + 2^2 + 2(x(-2y) + (-2y)2 + 2x)$$

$$= x^2 + 4y^2 + 4 + 2(-2xy - 4y + 2x)$$